---
id: 832
title: A Theorem on the Consumer Surplus
date: 2014-04-02T20:28:11-04:00
author: James Howard
layout: post
guid: http://beta.jameshoward.us/?p=832
permalink: /2014/04/02/a-theorem-on-the-consumer-surplus/
dsq_thread_id:
  - "2296631506"
bpxl_standard_single:
  - "0"
bpxl_audio_single:
  - "0"
bpxl_video_single:
  - "0"
bpxl_gallery_single:
  - "0"
bpxl_status_single:
  - "0"
bpxl_singlerelated:
  - "0"
categories:
  - Blog
tags:
  - demand
  - economic analysis
  - economics
  - environmental policy
  - environmental studies
  - flood studies
  - mathematics
  - statistics
---
<em>Theorem. Let [latex]m[/latex] be a scaling factor and [latex]y = \beta_0 + \beta_1 x_1 + \cdots[/latex] </em><em>be a generalized linear model such that [latex]y[/latex] is the amount of a good or </em><em>service purchased and [latex]x[/latex] is the price per unit of the good or </em><em>service. If [latex]y^\prime = \beta_0^\prime + \beta_1^\prime x_1^\prime + \cdots[/latex] such that [latex]y^\prime = my[/latex] and [latex]x_1^\prime = x_1 / m[/latex], then,
$$
-\frac{\hat{y}^{\prime\,2}}{2\hat{\beta_1^\prime}} =
-\frac{\hat{y}^2}{2\hat{\beta_1}} \label{eqn:thm} \text{.}
$$
</em>

If [latex]y^\prime = \beta_0^\ast + \beta_1^\ast x_1 + \cdots[/latex], then [latex]\beta_1^\ast = m\beta_1[/latex]. [1. Jeffrey Wooldridge, <i>Introductory econometrics: A modern approach,</i> Cengage Learning, 2012, p. 40.] Similarly, if [latex]y = \beta_0^\ast + \beta_1^\ast x_1^\prime + \cdots[/latex], then [latex]\beta_1^\ast = m\beta_1[/latex]. Therefore, if [latex]y^\prime = \beta_0^\prime + \beta_1^\prime x_1^\prime + \cdots[/latex], then [latex]\beta_1^\prime = m^2\beta_1[/latex]. Accordingly,
$$-\frac{\hat{y}^{\prime\,2}}{2\hat{\beta_1^\prime}} =
-\frac{(m\hat{y})^2}{2m^2\hat{\beta_1}} =
-\frac{m^2\hat{y}^2}{2m^2\hat{\beta_1}} =
-\frac{\hat{y}^2}{2\hat{\beta_1}} \text{.}
$$
